kruskal/spatial_wedgearray_graph.v
@@ -5,6 +5,7 @@ Require Import RamifyCoq.graph.FiniteGraph.
 Require Import VST.veric.SeparationLogic.
 Require Import RamifyCoq.kruskal.env_kruskal_edgelist.
 Require Import RamifyCoq.floyd_ext.share.
+Require Import RamifyCoq.kruskal.undirected_graph.
 
 Local Open Scope logic.
 
@@ -16,89 +17,35 @@ Definition wedge_to_cdata (wedge : LE*EType) : reptype t_struct_edge :=
   ).
 
 Lemma wedge_to_cdata_wedgerep:
-  forall w, Int.min_signed <= Int.signed (Int.repr (fst w)) <= Int.max_signed ->
-            Int.min_signed <= Int.signed (Int.repr (fst (snd w))) <= Int.max_signed ->
-            Int.min_signed <= Int.signed (Int.repr (snd (snd w))) <= Int.max_signed ->
+  forall w, Int.min_signed <= fst w <= Int.max_signed ->
+            Int.min_signed <= fst (snd w) <= Int.max_signed ->
+            Int.min_signed <= snd (snd w) <= Int.max_signed ->
             def_wedgerep (wedge_to_cdata w).
 Proof.
   intros. unfold wedge_to_cdata; unfold def_wedgerep; simpl. lia.
 Qed.
 
-Lemma def_wedgerep_map_w2c:
-  forall g,
-    Forall def_wedgerep (map wedge_to_cdata (graph_to_wedgelist g)).
+Definition c_connected_by_path g P p u v :=
+match u, v with
+| Vint u', Vint v' => connected_by_path g P p (Int.signed u') (Int.signed v')
+| _, _ => False
+end.
+
+Definition cdata_to_wedge (cwedge: reptype t_struct_edge) : option (LE*EType) :=
+match cwedge with
+| (Vint w, (Vint x, Vint y)) => Some (Int.signed w,(Int.signed x,Int.signed y))
+| _ => None
+end.
+
+Lemma w2c2w:
+  forall w, Int.min_signed <= fst w <= Int.max_signed ->
+            Int.min_signed <= fst (snd w) <= Int.max_signed ->
+            Int.min_signed <= snd (snd w) <= Int.max_signed ->
+            cdata_to_wedge (wedge_to_cdata w) = Some w.
 Proof.
-  intros.
-  rewrite Forall_forall; intros.
-  apply list_in_map_inv in H.
-  destruct H as [? [? _]].
-  unfold wedge_to_cdata in H.
-  unfold def_wedgerep.
-  rewrite (surjective_pairing x) in *.
-  inversion H; clear H.
-  destruct x.
-  rewrite (surjective_pairing c) in *.
-  simpl fst in *; simpl snd in *.
-  inversion H2; clear H2.
-  rewrite H1, H0, H3. split3; trivial.
+unfold wedge_to_cdata; unfold cdata_to_wedge; intros.
+repeat rewrite Int.signed_repr by auto. destruct w; destruct p; simpl; auto.
 Qed.
 
-(*I'm not sure what this is for
-Instance SWEGA_VST: SpatialWEdgeListGraphAssum mpred. Proof. refine (Build_SpatialWEdgeListGraphAssum _ _ _ _ _). Defined.
-
-Instance SWEG_VST (sh: share): SpatialWEdgeListGraph pointer_val mpred.
-Proof.
-  (*should I include graph->V and graph->E too? i.e. the full graph struct*)
-  (*I have no idea what the ordering of the lst is. Maybe I need Permutation or something*)
-  exact (fun pt lst => data_at sh (tarray t_struct_edge (Z.of_nat (length lst)))
-                              (map wedge_to_cdata lst) (pointer_val_val pt) (*I think this is wrong, should be just pt*)
-        ).
-Defined.
-*)
-Definition wedgearray_graph_rep sh (g: FiniteWEdgeListGraph) gptr eptr : mpred :=
-  data_at sh (t_wedgearray_graph) (
-    Vint (Int.repr (numV g)), (Vint (Int.repr (numE g)), pointer_val_val eptr)
-  ) (pointer_val_val gptr)
-  *
-  data_at sh (tarray t_struct_edge (numE g)) (map wedge_to_cdata (graph_to_wedgelist g)) (pointer_val_val eptr)
-  *
-  data_at sh (tarray t_struct_edge (MAX_EDGES - (numE g)))
-    (list_repeat (Z.to_nat MAX_EDGES - Z.to_nat (numE g)) (Vundef, (Vundef, Vundef)))
-    (offset_val ((numE g) * sizeof t_struct_edge) (pointer_val_val eptr))
-  .
-
-(* See if I need something like this next time
-Lemma graph_unfold: forall sh contents ptr i,
-    0 <= i < (Zlength contents) ->
-    graph_rep sh contents ptr =
-    iter_sepcon.iter_sepcon (list_rep sh MAX_EDGES ptr contents)
-            (sublist 0 i (nat_inc_list (Z.to_nat (Zlength contents)))) *
-    (list_rep sh MAX_EDGES ptr contents i *
-           iter_sepcon.iter_sepcon (list_rep sh MAX_EDGES ptr contents)
-             (sublist (i + 1) (Zlength contents) (nat_inc_list (Z.to_nat (Zlength contents))))).
-Proof.
-  intros. unfold graph_rep.
-  replace (nat_inc_list (Z.to_nat (Zlength contents))) with
-      (sublist 0 (Zlength contents) (nat_inc_list (Z.to_nat (Zlength contents)))) at 1.
-  2: { rewrite sublist_same; trivial.
-       rewrite nat_inc_list_Zlength, Z2Nat_id', Z.max_r; trivial.
-       apply Zlength_nonneg.
-  }
-  rewrite (sublist_split 0 i (Zlength contents)),
-  (sublist_split i (i+1) (Zlength contents)), (sublist_one i); try lia.
-  2, 3, 4: rewrite nat_inc_list_Zlength; rewrite Z2Nat.id; lia.
-  rewrite nat_inc_list_i.
-  2: rewrite Z2Nat_id', Z.max_r; trivial; apply Zlength_nonneg. 
-  repeat rewrite iter_sepcon.iter_sepcon_app.
-  simpl. rewrite sepcon_emp. reflexivity.
-Qed.
-*)
-
-(*
-Lemma graph_sep: forall sh graph ptr,
-    graph_rep sh graph ptr =
-	data_at tint (numV g) ptr *
-	data_at tint (numE g) (?) *
-	SWEG_VST (?) (graph_to_wedgelist graph).
-Proof.
-*)
+Definition Vundef_cwedges n: list (reptype t_struct_edge) :=
+    list_repeat n (Vundef, (Vundef, Vundef)).
